semantics/proofs/semanticPrimitivesPropsScript.sml
@@ -365,7 +365,7 @@ val do_opapp_cases = store_thm("do_opapp_cases",
 val build_rec_env_help_lem = Q.prove (
   `∀funs env funs'.
     FOLDR (λ(f,x,e) env'. eBind f (Recclosure env funs' f) env') env' funs =
-    eMerge (alist_to_env (MAP (λ(f,n,e). (f, Recclosure env funs' f)) funs)) env'`,
+    eAppend (alist_to_env (MAP (λ(f,n,e). (f, Recclosure env funs' f)) funs)) env'`,
  Induct >>
  srw_tac[][] >>
  PairCases_on `h` >>
@@ -375,7 +375,7 @@ val build_rec_env_help_lem = Q.prove (
 val build_rec_env_merge = Q.store_thm ("build_rec_env_merge",
 `∀funs funs' env env'.
   build_rec_env funs env env' =
-  eMerge (alist_to_env (MAP (λ(f,n,e). (f, Recclosure env funs f)) funs)) env'`,
+  eAppend (alist_to_env (MAP (λ(f,n,e). (f, Recclosure env funs f)) funs)) env'`,
 srw_tac[][build_rec_env_def, build_rec_env_help_lem]);
 
 val do_con_check_build_conv = Q.store_thm ("do_con_check_build_conv",
@@ -424,7 +424,7 @@ val same_tid_tid = Q.store_thm("same_tid_tid",
 val build_tdefs_cons = Q.store_thm ("build_tdefs_cons",
 `(!tvs tn ctors tds mn.
   build_tdefs mn ((tvs,tn,ctors)::tds) =
-    eMerge (build_tdefs mn tds)
+    eAppend (build_tdefs mn tds)
            (alist_to_env (REVERSE (MAP (\(conN,ts). (conN, LENGTH ts, TypeId (mk_id mn tn))) ctors)))) ∧
  (!mn. build_tdefs mn [] = eEmpty)`,
  srw_tac[][build_tdefs_def, REVERSE_APPEND]);
